

# Backpropagation via Computation Graphs

A Complete Worked Example for a 2-Layer Neural Network

## 1. Overview

This document walks through backpropagation for a simple 2-layer neural network (2 inputs, 2 hidden units, 1 output). We treat the network as a **computation graph** where values flow forward and gradients flow backward.

## 2. The Computation Graph

The network can be visualised as a chain of operations:

$$x \rightarrow z1 \xrightarrow{(W1)} a1 \xrightarrow{(s)} z2 \xrightarrow{(W2)} a2 \xrightarrow{(s)} L$$

More explicitly, in vector form:

$$x \rightarrow z1 = W1*x + b1 \rightarrow a1 = \text{sigma}(z1) \\ \downarrow v \\ z2 = W2*a1 + b2 \rightarrow a2 = \text{sigma}(z2) \rightarrow L$$

## 3. Forward Pass: Values Flow Left to Right

During the forward pass, we compute and **store** all intermediate values. These cached values will be needed during backpropagation.

### Step-by-step computations:

Step	Node	Computation
1	Linear (hidden)	$z1 = W1*x + b1$
2	Activation (hidden)	$a1 = \text{sigma}(z1)$
3	Linear (output)	$z2 = W2*a1 + b2$
4	Activation (output)	$a2 = \text{sigma}(z2)$
5	Loss	$L = (1/2)*(a2 - y)^2$

## 4. Backward Pass: Gradients Flow Right to Left

Each node asks: "How does the loss change if I change slightly?" We apply the chain rule at each node, propagating gradients backward.

## 4.1 Loss to Output Activation

Starting at the loss node:

$$dL/da_2 = a_2 - y$$

## 4.2 Output Activation to Output Pre-activation

Since  $a_2 = \sigma(z_2)$ , by the chain rule:

$$da_2/dz_2 = \sigma'(z_2)$$

Combining these gives the **output error signal**:

$$\delta_2 = dL/dz_2 = (dL/da_2) * (da_2/dz_2) = (a_2 - y) * \sigma'(z_2)$$

## 4.3 Output Pre-activation to Weights, Bias, and Hidden Activations

Since  $z_2 = W_2 * a_1 + b_2$ , the gradient branches to three destinations:

Destination	Gradient Formula
Weight $W_2$	$dL/dW_2 = \delta_2 * a_1^T$
Bias $b_2$	$dL/db_2 = \delta_2$
Hidden activation $a_1$	$dL/da_1 = W_2^T * \delta_2$

## 4.4 Hidden Activation to Hidden Pre-activation

Since  $a_1 = \sigma(z_1)$ :

$$da_1/dz_1 = \sigma'(z_1)$$

Applying the chain rule node-by-node gives the **hidden error signal**:

$$\delta_1 = dL/dz_1 = (W_2^T * \delta_2) [\text{elementwise*}] \sigma'(z_1)$$

This is where  $\delta_1$  comes from: it is the gradient at the  $z_1$  node, computed by propagating  $\delta_2$  backward through the weight matrix and element-wise multiplying by the local derivative of the activation.

## 4.5 Hidden Pre-activation to First-Layer Parameters

Since  $z_1 = W_1 * x + b_1$ :

Parameter	Gradient Formula
Weight $W_1$	$dL/dW_1 = \delta_1 * x^T$

Bias b1	$dL/db1 = \text{delta1}$
---------	--------------------------

## 5. Summary of Error Signals

Symbol	Node	Formula	Meaning
delta2	z2	$(a2 - y) * \sigma'(z2)$	Output layer error
delta1	z1	$(W2^T * \text{delta2}) [\text{elem}^*] \sigma'(z1)$	Hidden layer error

## 6. Key Insights

### delta1 is not arbitrary

It is precisely  $dL/dz1$  - the gradient of the loss with respect to the hidden layer's pre-activation. It arises naturally from traversing the computation graph backward.

### Backprop is reverse graph traversal

The forward pass computes values; the backward pass computes derivatives. Same graph, opposite direction.

### Every delta corresponds to a node

Each error signal  $\text{delta}_k$  represents the gradient at a specific pre-activation node  $z_k$ . This is why error signals propagate - they follow the graph structure.

*"Backpropagation is just the chain rule applied to a computation graph, one node at a time, from right to left."*